More saturn/mpmc_bqueue.

theories/saturn/mpmc_bqueue.v
@@ -7,6 +7,10 @@ From iris.base_logic Require Import
 
 From zoo Require Import
   prelude.
+From zoo.common Require Import
+  list.
+From zoo.iris.bi Require Import
+  big_op.
 From zoo.iris.base_logic Require Import
   lib.mono_list
   lib.auth_nat_max
@@ -69,24 +73,30 @@ Definition mpmc_bqueue_is_empty : val :=
     if: "new_back".{xchain_next} = () and ~ CAS "t".[back] "back" "new_back" then
       "mpmc_bqueue_fix_back" "t" "t".{back} "new_back".
 #[local] Definition mpmc_bqueue_do_push : val :=
-  rec: "mpmc_bqueue_do_push" "t" "back" "new_back" "cap" =>
+  rec: "mpmc_bqueue_do_push" "t" "node" "new_back" "cap" =>
     if: "cap" = #0 then (
-      let: "cap" := "t".{capacity} - ("back".{xchain_index} - "t".{front}.{xchain_index}) in
+      let: "cap" := "t".{capacity} - ("node".{xchain_index} - "t".{front}.{xchain_index}) in
       if: "cap" ≤ #0 then (
         #false
       ) else (
-        "back" <-{xchain_capacity} "cap" ;;
-        "mpmc_bqueue_do_push" "t" "back" "new_back" "cap"
+        "node" <-{xchain_capacity} "cap" ;;
+        "mpmc_bqueue_do_push" "t" "node" "new_back" "cap"
       )
     ) else (
       "new_back" <-{xchain_capacity} "cap" - #1 ;;
-      "new_back" <-{xchain_index} #1 + "back".{xchain_index} ;;
-      if: CAS "back".[xchain_next] () "new_back" then (
-        mpmc_bqueue_fix_back "t" "back" "new_back" ;;
-        #true
+      "new_back" <-{xchain_index} #1 + "node".{xchain_index} ;;
+      let: "node'" := "node".{xchain_next} in
+      if: "node'" = () then (
+        if: CAS "node".[xchain_next] () "new_back" then (
+          mpmc_bqueue_fix_back "t" "node" "new_back" ;;
+          #true
+        ) else (
+          Yield ;;
+          let: "node'" := "node".{xchain_next} in
+          "mpmc_bqueue_do_push" "t" "node'" "new_back" "node'".{xchain_capacity}
+        )
       ) else (
-        let: "back" := "back".{xchain_next} in
-        "mpmc_bqueue_do_push" "t" "back" "new_back" "back".{xchain_capacity}
+          "mpmc_bqueue_do_push" "t" "node'" "new_back" "node'".{xchain_capacity}
       )
     ).
 Definition mpmc_bqueue_push : val :=
@@ -101,15 +111,13 @@ Definition mpmc_bqueue_pop : val :=
     let: "front" := "old_front".{xchain_next} in
     if: "front" = () then (
       §None
+    ) else if: CAS "t".[front] "old_front" "front" then (
+      let: "v" := "front".{xchain_data} in
+      "front" <-{xchain_data} () ;;
+      ‘Some( "v" )
     ) else (
-      if: CAS "t".[front] "old_front" "front" then (
-        let: "v" := "front".{xchain_data} in
-        "front" <-{xchain_data} () ;;
-        ‘Some( "v" )
-      ) else (
-        Yield ;;
-        "mpmc_bqueue_pop" "t"
-      )
+      Yield ;;
+      "mpmc_bqueue_pop" "t"
     ).
 
 Class MpmcBqueueG Σ `{zoo_G : !ZooG Σ} := {
@@ -224,11 +232,11 @@ Section mpmc_bqueue_G.
     ( [∗ list] node; v ∈ nodes; vs,
       node.[xchain_data] ↦ v
     ) ∗
-    ( [∗ list] i ↦ node ∈ past ++ front :: nodes,
-      ∃ cap,
-      ⌜i + cap ≤ length past + γ.(mpmc_bqueue_meta_capacity)⌝ ∗
-      node.[xchain_index] ↦ #i ∗
-      node.[xchain_capacity] ↦ #cap
+    ( [∗ list] i ↦ node ∈ hist,
+      ∃ (cap : nat),
+      node.[xchain_index] ↦□ #i ∗
+      node.[xchain_capacity] ↦ #cap ∗
+      ⌜i + cap ≤ length past + γ.(mpmc_bqueue_meta_capacity)⌝
     ) ∗
     mpmc_bqueue_history_auth γ hist ∗
     mpmc_bqueue_front_auth γ (length past) ∗
@@ -241,13 +249,14 @@ Section mpmc_bqueue_G.
     ∃ l γ,
     ⌜t = #l⌝ ∗
     ⌜cap = γ.(mpmc_bqueue_meta_capacity)⌝ ∗
-    l.[capacity] ↦□ #cap ∗
     meta l nroot γ ∗
+    l.[capacity] ↦□ #cap ∗
     inv ι (mpmc_bqueue_inv_inner l γ ι).
 
   Definition mpmc_bqueue_model t vs : iProp Σ :=
     ∃ l γ,
     ⌜t = #l⌝ ∗
+    ⌜length vs ≤ γ.(mpmc_bqueue_meta_capacity)⌝ ∗
     meta l nroot γ ∗
     mpmc_bqueue_model₁ γ vs.
 
@@ -374,6 +383,16 @@ Section mpmc_bqueue_G.
     apply ghost_map_delete.
   Qed.
 
+  Lemma mpmc_bqueue_model_valid t ι cap vs :
+    mpmc_bqueue_inv t ι cap -∗
+    mpmc_bqueue_model t vs -∗
+    ⌜length vs ≤ cap⌝.
+  Proof.
+    iIntros "(%l & %γ & -> & -> & #Hmeta & #Hl_capacity & #Hinv) (%_l & %_γ & %Heq & %Hvs & #_Hmeta & Hmodel₁)". injection Heq as <-.
+    iDestruct (meta_agree with "Hmeta _Hmeta") as %<-. iClear "_Hmeta".
+    iSteps.
+  Qed.
+
   Lemma mpmc_bqueue_create_spec ι cap :
     (0 ≤ cap)%Z →
     {{{ True }}}
@@ -389,6 +408,7 @@ Section mpmc_bqueue_G.
     wp_rec.
 
     wp_block front as "(Hfront_next & Hfront_data & Hfront_index & Hfront_capacity & _)".
+    iMod (pointsto_persist with "Hfront_index") as "#Hfront_index".
     wp_block l as "Hmeta" "(Hl_capacity & Hl_front & Hl_back & _)".
     iMod (pointsto_persist with "Hl_capacity") as "#Hcapacity".
     rewrite -{1 3}(Z2Nat.id cap) //.
@@ -413,7 +433,288 @@ Section mpmc_bqueue_G.
     iExists l, γ. iStep 4. iApply inv_alloc.
     iExists [front], [], front, [], front, [], ∅. iFrame. iSteps.
     - rewrite elem_of_list_singleton //.
-    - iExists (Z.to_nat cap). iSteps. rewrite big_sepM_empty //.
+    - rewrite big_sepM_empty //.
+  Qed.
+
+  Lemma mpmc_bqueue_capacity_spec t ι cap :
+    {{{
+      mpmc_bqueue_inv t ι cap
+    }}}
+      mpmc_bqueue_capacity t
+    {{{
+      RET #cap;
+      True
+    }}}.
+  Proof.
+    iSteps.
+  Qed.
+
+  #[local] Lemma mpmc_bqueue_front_spec_strong au Ψ l γ ι :
+    {{{
+      inv ι (mpmc_bqueue_inv_inner l γ ι) ∗
+      if negb au then True else
+        mpmc_bqueue_waiter_au γ ι Ψ
+    }}}
+      (#l).{front}
+    {{{ front i,
+      RET #front;
+      mpmc_bqueue_history_elem γ i front ∗
+      front.[xchain_index] ↦□ #i ∗
+      mpmc_bqueue_front_lb γ i ∗
+      if negb au then True else
+        ∃ waiter,
+        saved_pred waiter Ψ ∗
+        mpmc_bqueue_waiters_frag γ waiter i
+    }}}.
+  Proof.
+    iIntros "%Φ (#Hinv & HΨ) HΦ".
+
+    iInv "Hinv" as "(%hist & %past & %front & %nodes & %back & %vs & %waiters & >%Hhist & >%Hback & Hl_front & Hl_back & Hhist & Hnodes & Hindexing & Hhistory_auth & Hfront_auth & Hmodel₂ & Hwaiters_auth & Hwaiters)".
+    wp_load.
+    assert (hist !! length past = Some front) as Hhist_lookup.
+    { rewrite Hhist list_lookup_middle //. }
+    iDestruct (mpmc_bqueue_history_elem_get _ front with "Hhistory_auth") as "#Hhistory_elem"; first done.
+    iAssert (front.[xchain_index] ↦□ #(length past))%I as "#Hfront_index".
+    { rewrite big_sepL_lookup //. iSteps. }
+    iDestruct (mpmc_bqueue_front_lb_get with "Hfront_auth") as "#Hfront_lb".
+    destruct au.
+
+    - iMod (saved_pred_alloc_cofinite (dom waiters) Ψ) as "(%waiter & %Hwaiter & #Hwaiter)".
+      rewrite not_elem_of_dom in Hwaiter.
+      iMod (mpmc_bqueue_waiters_insert _ (length past) with "Hwaiters_auth") as "(Hwaiter_auth & Hwaiters_frag)"; first done.
+      iDestruct (big_sepM_insert_2 _ _ waiter (length past) with "[HΨ] Hwaiters") as "Hwaiters".
+      { iExists Ψ. rewrite decide_False; first lia. iSteps. }
+      iSplitR "Hwaiters_frag HΦ". { repeat iExists _. iSteps. }
+      iSteps.
+
+    - iSplitR "HΦ". { repeat iExists _. iSteps. }
+      iSteps.
+  Qed.
+  #[local] Lemma mpmc_bqueue_front_spec l γ ι :
+    {{{
+      inv ι (mpmc_bqueue_inv_inner l γ ι)
+    }}}
+      (#l).{front}
+    {{{ front i,
+      RET #front;
+      mpmc_bqueue_history_elem γ i front ∗
+      front.[xchain_index] ↦□ #i ∗
+      mpmc_bqueue_front_lb γ i
+    }}}.
+  Proof.
+    iIntros "%Φ #Hinv HΦ".
+    wp_apply (mpmc_bqueue_front_spec_strong false inhabitant with "[$Hinv]").
+    iSteps.
+  Qed.
+
+  #[local] Lemma mpmc_bqueue_back_spec l γ ι :
+    {{{
+      inv ι (mpmc_bqueue_inv_inner l γ ι)
+    }}}
+      (#l).{back}
+    {{{ back i,
+      RET #back;
+      mpmc_bqueue_history_elem γ i back ∗
+      back.[xchain_index] ↦□ #i
+    }}}.
+  Proof.
+    iIntros "%Φ #Hinv HΦ".
+
+    iInv "Hinv" as "(%hist & %past & %front & %nodes & %back & %vs & %waiters & >%Hhist & >%Hback & Hl_front & Hl_back & Hhist & Hnodes & Hindexing & Hhistory_auth & Hfront_auth & Hmodel₂ & Hwaiters_auth & Hwaiters)".
+    wp_load.
+    pose proof Hback as (i & Hlookup)%elem_of_list_lookup.
+    iDestruct (mpmc_bqueue_history_elem_get with "Hhistory_auth") as "#Hhistory_elem_back"; first done.
+    iAssert (back.[xchain_index] ↦□ #i)%I as "#Hback_index".
+    { rewrite big_sepL_lookup //. iSteps. }
+    iSplitR "HΦ". { repeat iExists _. iSteps. }
+    iSteps.
+  Qed.
+
+  Inductive mpmc_bqueue_op :=
+    | MpmcQueueIsEmpty
+    | MpmcQueuePop
+    | MpmcQueueOther.
+  #[local] Instance mpmc_bqueue_op_eq_dec : EqDecision mpmc_bqueue_op :=
+    ltac:(solve_decision).
+
+  #[local] Lemma mpmc_bqueue_xchain_next_spec_strong op TB waiter Ψ_is_empty β x Ψ_pop l γ ι i node :
+    {{{
+      meta l nroot γ ∗
+      inv ι (mpmc_bqueue_inv_inner l γ ι) ∗
+      mpmc_bqueue_history_elem γ i node ∗
+      if decide (op = MpmcQueueOther) then True else
+        mpmc_bqueue_front_lb γ i ∗
+        if decide (op = MpmcQueueIsEmpty) then
+          saved_pred waiter Ψ_is_empty ∗
+          mpmc_bqueue_waiters_frag γ waiter i ∗
+          £ 1
+        else
+          atomic_update (TA := [tele vs]) (TB := TB) (⊤ ∖ ↑ι) ∅ (tele_app $ mpmc_bqueue_model #l) β Ψ_pop ∗
+          ( mpmc_bqueue_model #l [] -∗
+            β [tele_arg []] x
+          )
+    }}}
+      (#node).{xchain_next}
+    {{{ res,
+      RET res;
+      ( ⌜res = ()%V⌝ ∗
+        match op with
+        | MpmcQueueIsEmpty =>
+            Ψ_is_empty true
+        | MpmcQueuePop =>
+            Ψ_pop [tele_arg []] x
+        | MpmcQueueOther =>
+            True
+        end
+      ) ∨ (
+        ∃ node',
+        ⌜res = #node'⌝ ∗
+        mpmc_bqueue_history_elem γ (S i) node' ∗
+        node'.[xchain_index] ↦□ #(S i) ∗
+        match op with
+        | MpmcQueueIsEmpty =>
+            Ψ_is_empty false
+        | MpmcQueuePop =>
+            atomic_update (TA := [tele vs]) (TB := TB) (⊤ ∖ ↑ι) ∅ (tele_app $ mpmc_bqueue_model #l) β Ψ_pop
+        | MpmcQueueOther =>
+            True
+        end
+      )
+    }}}.
+  Proof.
+    iIntros "%Φ (#Hmeta & #Hinv & #Hhistory_elem & Hop) HΦ".
+
+    iInv "Hinv" as "(%hist & %past & %front & %nodes & %back & %vs & %waiters & >%Hhist & >%Hback & Hl_front & Hl_back & Hhist & Hnodes & Hindexing & >Hhistory_auth & Hfront_auth & Hmodel₂ & Hwaiters_auth & Hwaiters)".
+    iDestruct (mpmc_bqueue_history_agree with "Hhistory_auth Hhistory_elem") as %Hlookup.
+    iDestruct (xchain_model_lookup_acc with "Hhist") as "(Hnode & Hhist)"; first done.
+    wp_load.
+    iDestruct ("Hhist" with "Hnode ") as "Hhist".
+    destruct (hist !! S i) as [node' |] eqn:Hlookup'; simpl.
+
+    - iDestruct (mpmc_bqueue_history_elem_get (S i) with "Hhistory_auth") as "#Hhistory_elem'"; first done.
+      iAssert (node'.[xchain_index] ↦□ #(S i))%I as "#Hnode'_index".
+      { rewrite big_sepL_lookup //. iSteps. }
+      destruct op.
+
+      + iDestruct "Hop" as "(#Hfront_lb & #Hwaiter & Hwaiters_frag & H£)".
+        iDestruct (mpmc_bqueue_waiters_lookup with "Hwaiters_auth Hwaiters_frag") as %Hwaiters_lookup.
+        iMod (mpmc_bqueue_waiters_delete with "Hwaiters_auth Hwaiters_frag") as "Hwaiters_auth".
+        iDestruct (big_sepM_delete with "Hwaiters") as "((%Ψ & _Hwaiter & HΨ) & Hwaiters)"; first done.
+        iDestruct (saved_pred_agree false with "Hwaiter _Hwaiter") as "HΨ_is_empty".
+        iMod (lc_fupd_elim_later with "H£ HΨ_is_empty") as "HΨ_is_empty".
+        destruct (decide (i = length past)) as [-> | Hi].
+
+        * rewrite decide_False; first lia.
+          iMod "HΨ" as "(%_vs & Hmodel₁ & _ & HΨ)".
+          iDestruct (mpmc_bqueue_model_agree with "Hmodel₁ Hmodel₂") as %->.
+          iMod ("HΨ" with "Hmodel₁") as "HΨ".
+          assert (nodes ≠ []) as Hnodes.
+          { apply lookup_lt_Some in Hlookup'.
+            rewrite Hhist app_length /= in Hlookup'.
+            naive_solver lia.
+          }
+          iAssert ⌜vs ≠ []⌝%I as %Hvs.
+          { destruct (decide (vs = [])) as [-> |]; last done.
+            iDestruct (big_sepL2_length with "Hnodes") as %->%nil_length_inv.
+            iSteps.
+          }
+          rewrite bool_decide_eq_false_2 //.
+          iSplitR "HΨ_is_empty HΨ HΦ". { repeat iExists _. iFrame. iSteps. }
+          iSteps. iRewrite "HΨ_is_empty". iSteps.
+
+        * iDestruct (mpmc_bqueue_front_lb_valid with "Hfront_auth Hfront_lb") as %Hi_.
+          rewrite decide_True; first lia.
+          iSplitR "HΨ_is_empty HΨ HΦ". { repeat iExists _. iFrame. iSteps. }
+          iSteps. iRewrite "HΨ_is_empty". iSteps.
+
+      + iSplitR "Hop HΦ". { repeat iExists _. iSteps. }
+        iSteps.
+
+      + iSplitR "Hop HΦ". { repeat iExists _. iSteps. }
+        iSteps.
+
+    - destruct (decide (op = MpmcQueueOther)) as [-> | Hop].
+
+      + iSplitR "HΦ". { repeat iExists _. iSteps. }
+        iSteps.
+
+      + iDestruct "Hop" as "(#Hfront_lb & Hop)".
+        iDestruct (mpmc_bqueue_front_lb_valid with "Hfront_auth Hfront_lb") as %Hi.
+        opose proof* lookup_last_length as Hlength; [done.. |].
+        rewrite Hhist app_length /= in Hlength.
+        assert (i = length past) as -> by lia.
+        assert (length nodes = 0) as ->%nil_length_inv by lia.
+        iDestruct (big_sepL2_length with "Hnodes") as %->%symmetry%nil_length_inv.
+        destruct op; last done.
+
+        * iDestruct "Hop" as "(#Hwaiter & Hwaiters_frag & H£)".
+          iDestruct (mpmc_bqueue_waiters_lookup with "Hwaiters_auth Hwaiters_frag") as %Hwaiters_lookup.
+          iMod (mpmc_bqueue_waiters_delete with "Hwaiters_auth Hwaiters_frag") as "Hwaiters_auth".
+          iDestruct (big_sepM_delete with "Hwaiters") as "((%Ψ & _Hwaiter & HΨ) & Hwaiters)"; first done.
+          iDestruct (saved_pred_agree true with "Hwaiter _Hwaiter") as "HΨ_is_empty".
+          iMod (lc_fupd_elim_later with "H£ HΨ_is_empty") as "HΨ_is_empty".
+          rewrite decide_False; first lia.
+          iMod "HΨ" as "(%vs & Hmodel₁ & _ & HΨ)".
+          iDestruct (mpmc_bqueue_model_agree with "Hmodel₁ Hmodel₂") as %->.
+          iMod ("HΨ" with "Hmodel₁") as "HΨ".
+          iSplitR "HΨ_is_empty HΨ HΦ". { repeat iExists _. iFrame. iSteps. }
+          iModIntro. clear.
+
+          iApply "HΦ".
+          iLeft. iRewrite "HΨ_is_empty". iSteps.
+
+        * iDestruct "Hop" as "(HΨ & Hβ)".
+          iMod "HΨ" as "(%vs & (%_l & %_γ & %Heq & %Hvs & #_Hmeta & Hmodel₁) & _ & HΨ)". injection Heq as <-.
+          iDestruct (meta_agree with "Hmeta _Hmeta") as %<-. iClear "_Hmeta".
+          iDestruct (mpmc_bqueue_model_agree with "Hmodel₁ Hmodel₂") as %->.
+          iDestruct ("Hβ" with "[Hmodel₁]") as "Hβ"; first iSteps.
+          iMod ("HΨ" with "Hβ") as "HΨ".
+          iSplitR "HΨ HΦ". { repeat iExists _. iFrame. iSteps. }
+          iSteps.
+  Qed.
+  #[local] Lemma mpmc_bqueue_xchain_next_spec l γ ι i node :
+    {{{
+      meta l nroot γ ∗
+      inv ι (mpmc_bqueue_inv_inner l γ ι) ∗
+      mpmc_bqueue_history_elem γ i node
+    }}}
+      (#node).{xchain_next}
+    {{{ res,
+      RET res;
+        ⌜res = ()%V⌝
+      ∨ ∃ node',
+        ⌜res = #node'⌝ ∗
+        mpmc_bqueue_history_elem γ (S i) node' ∗
+        node'.[xchain_index] ↦□ #(S i)
+    }}}.
+  Proof.
+    iIntros "%Φ (#Hmeta & #Hinv & #Hhistory_elem) HΦ".
+    wp_apply (mpmc_bqueue_xchain_next_spec_strong MpmcQueueOther TeleO inhabitant inhabitant inhabitant inhabitant inhabitant with "[$]").
+    iSteps.
+  Qed.
+
+  #[local] Lemma mpmc_bqueue_xchain_capacity l γ ι i node:
+    {{{
+      meta l nroot γ ∗
+      inv ι (mpmc_bqueue_inv_inner l γ ι) ∗
+      mpmc_bqueue_history_elem γ i node
+    }}}
+      (#node).{xchain_capacity}
+    {{{ cap j,
+      RET #cap;
+      ⌜i + cap ≤ j + γ.(mpmc_bqueue_meta_capacity)⌝ ∗
+      mpmc_bqueue_front_lb γ j
+    }}}.
+  Proof.
+    iIntros "%Φ (#Hmeta & #Hinv & #Hhistory_elem) HΦ".
+    iInv "Hinv" as "(%hist & %past & %front & %nodes & %back & %vs & %waiters & >%Hhist & >%Hback & Hl_front & Hl_back & Hhist & Hnodes & Hindexing & >Hhistory_auth & Hfront_auth & Hmodel₂ & Hwaiters_auth & Hwaiters)".
+    iDestruct (mpmc_bqueue_history_agree with "Hhistory_auth Hhistory_elem") as %Hlookup.
+    iDestruct (big_sepL_lookup_acc with "Hindexing") as "((%cap & Hnode_index & Hnode_capacity & >%) & Hindexing)"; first done.
+    wp_load.
+    iDestruct (mpmc_bqueue_front_lb_get with "Hfront_auth") as "#Hfront_lb".
+    iDestruct ("Hindexing" with "[Hnode_index Hnode_capacity]") as "Hindexing"; first iSteps.
+    iSplitR "HΦ". { repeat iExists _. iFrame. iSteps. }
+    iSteps.
   Qed.
 
   Lemma mpmc_bqueue_is_empty_spec t ι cap :
@@ -422,13 +723,133 @@ Section mpmc_bqueue_G.
     | ∀∀ vs,
       mpmc_bqueue_model t vs
     >>>
-      mpmc_bqueue_is_empty t
+      mpmc_bqueue_is_empty t @ ↑ι
     <<<
       mpmc_bqueue_model t vs
-    | RET #(bool_decide (vs = [])); True
+    | RET #(bool_decide (vs = []));
+      True
     >>>.
   Proof.
-  Admitted.
+    iIntros "!> %Φ (%l & %γ & -> & -> & #Hmeta & #Hl_capacity & #Hinv) HΦ".
+
+    wp_rec credit:"H£".
+    wp_smart_apply (mpmc_bqueue_front_spec_strong true (λ b, Φ #b) with "[$Hinv HΦ]") as (node i) "(#Hhistory_elem & #Hfront_index & #Hfront_lb & %waiter & #Hwaiter & Hwaiters_frag)".
+    { rewrite /= /mpmc_bqueue_waiter_au. iAuIntro.
+      iApply (aacc_aupd_commit with "HΦ"); first done. iIntros "%vs (%_l & %_γ & %Heq & %Hvs & #_Hmeta & Hmodel₁)". injection Heq as <-.
+      iDestruct (meta_agree with "Hmeta _Hmeta") as %<-. iClear "_Hmeta".
+      iAaccIntro with "Hmodel₁"; iSteps.
+    }
+    wp_smart_apply (mpmc_bqueue_xchain_next_spec_strong MpmcQueueIsEmpty [tele_pair bool] _ _ inhabitant [tele_arg true] inhabitant with "[$Hmeta $Hinv $Hhistory_elem $Hfront_lb $Hwaiter $Hwaiters_frag $H£]") as (res) "[(-> & HΦ) | (%node' & -> & #Hhistory_elem' & HΦ)]"; iSteps.
+  Qed.
+
+  #[local] Lemma mpmc_bqueue_fix_back_spec l γ ι i back j new_back :
+    {{{
+      meta l nroot γ ∗
+      inv ι (mpmc_bqueue_inv_inner l γ ι) ∗
+      mpmc_bqueue_history_elem γ i back ∗
+      mpmc_bqueue_history_elem γ j new_back
+    }}}
+      mpmc_bqueue_fix_back #l #back #new_back
+    {{{
+      RET ();
+      True
+    }}}.
+  Proof.
+    iIntros "%Φ (#Hmeta & #Hinv & #Hhistory_elem_back & #Hhistory_elem_new_back) HΦ".
+
+    iLöb as "HLöb" forall (i back) "Hhistory_elem_back".
+
+    wp_rec. wp_pures.
+    wp_bind (_ and _)%E.
+    wp_apply (wp_wand _ _ (λ res, ∃ b, ⌜res = #b⌝)%I) as (res) "(%b & ->)".
+    { wp_smart_apply (mpmc_bqueue_xchain_next_spec with "[$Hmeta $Hinv $Hhistory_elem_new_back]") as (res) "[-> | (%new_back' & -> & #Hhistory_elem_new_back')]"; last iSteps.
+      wp_pures.
+
+      wp_bind (CAS _ _ _).
+      iInv "Hinv" as "(%hist & %past & %front & %nodes & %back' & %vs & %waiters & >%Hhist & >%Hback & Hl_front & Hl_back & Hhist & Hnodes & Hindexing & Hhistory_auth & Hfront_auth & Hmodel₂ & Hwaiters_auth & Hwaiters)".
+      wp_cas as _ | [= ->].
+      2: iDestruct (mpmc_bqueue_history_agree with "Hhistory_auth Hhistory_elem_new_back") as %Hnew_back%elem_of_list_lookup_2.
+      all: iSplitL; first (repeat iExists _; iSteps).
+      all: iSteps.
+    }
+    destruct b; last iSteps.
+    wp_smart_apply (mpmc_bqueue_back_spec with "Hinv") as (back' i') "(#Hhistory_elem_back' & _)".
+    iApply ("HLöb" with "HΦ Hhistory_elem_back'").
+  Qed.
+
+  #[local] Lemma mpmc_bqueue_do_push_spec l γ ι i node new_back (cap : nat) j v v_index :
+    i + cap ≤ j + γ.(mpmc_bqueue_meta_capacity) →
+    <<<
+      meta l nroot γ ∗
+      l.[capacity] ↦□ #γ.(mpmc_bqueue_meta_capacity) ∗
+      inv ι (mpmc_bqueue_inv_inner l γ ι) ∗
+      mpmc_bqueue_history_elem γ i node ∗
+      node.[xchain_index] ↦□ #i ∗
+      new_back.[xchain_next] ↦ () ∗
+      new_back.[xchain_data] ↦ v ∗
+      new_back.[xchain_index] ↦ v_index ∗
+      new_back.[xchain_capacity] ↦ #cap ∗
+      mpmc_bqueue_front_lb γ j
+    | ∀∀ vs,
+      mpmc_bqueue_model #l vs
+    >>>
+      mpmc_bqueue_do_push #l #node #new_back #cap @ ↑ι
+    <<<
+      ∃∃ b,
+      if b then
+        mpmc_bqueue_model #l (vs ++ [v])
+      else
+        mpmc_bqueue_model #l vs
+    | RET #b;
+      True
+    >>>.
+  Proof.
+    iIntros "%Hcap !> %Φ (#Hmeta & #Hl_capacity & #Hinv & #Hhistory_elem & #Hnode_index & Hnew_back_next & Hnew_back_data & Hnew_back_index & Hnew_back_capacity & #Hfront_lb) HΦ".
+
+    iLöb as "HLöb" forall (i node cap Hcap) "Hhistory_elem Hnode_index".
+
+    wp_rec. wp_pures.
+    case_bool_decide as Hcase; wp_pures.
+
+    - admit.
+
+    - wp_store. wp_load. wp_store.
+      wp_smart_apply (mpmc_bqueue_xchain_next_spec with "[$Hmeta $Hinv $Hhistory_elem]") as (res) "[-> | (%node' & -> & #Hhistory_elem')]".
+
+      + wp_pures.
+
+        wp_bind (CAS _ _ _).
+        iInv "Hinv" as "(%hist & %past & %front & %nodes & %back & %vs & %waiters & >%Hhist & >%Hback & Hl_front & Hl_back & Hhist & Hnodes & Hindexing & >Hhistory_auth & Hfront_auth & Hmodel₂ & Hwaiters_auth & Hwaiters)".
+        iDestruct (mpmc_bqueue_history_agree with "Hhistory_auth Hhistory_elem") as %Hlookup.
+        iDestruct (xchain_model_lookup with "Hhist") as "(Hhist1 & Hnode & Hhist2)"; first done.
+        destruct (hist !! S i) as [node' |] eqn:Hlookup'; simpl.
+
+        * wp_cas as _ | [=].
+          iDestruct (xchain_model_lookup_2 with "Hhist1 Hnode Hhist2") as "Hhist"; [done | rewrite Hlookup' // |].
+          iSplitR "Hnew_back_next Hnew_back_data HΦ". { repeat iExists _. iSteps. }
+          iSteps.
+
+        * wp_cas as Hcas | _; first done.
+          iDestruct (xchain_model_lookup_2 with "Hhist1 Hnode []") as "Hhist"; [done | rewrite Hlookup' // | ..].
+          { rewrite -(lookup_last_length hist i) // drop_all //. }
+          iDestruct (big_sepL2_snoc with "[$Hnodes $Hnew_back_data]") as "Hnodes".
+          iDestruct (xchain_model_snoc_2 with "Hhist Hnew_back_next") as "Hhist".
+          iMod (mpmc_bqueue_history_update new_back with "Hhistory_auth") as "Hhistory_auth".
+          iDestruct (mpmc_bqueue_history_elem_get with "Hhistory_auth") as "#Hhistory_elem_new_back".
+          { rewrite lookup_snoc_Some. naive_solver. }
+          iMod "HΦ" as "(%_vs & (%_l & %_γ & %Heq & #_Hmeta & Hmodel₁) & _ & HΦ)". injection Heq as <-.
+          iDestruct (meta_agree with "Hmeta _Hmeta") as %<-. iClear "_Hmeta".
+          iDestruct (mpmc_bqueue_model_agree with "Hmodel₁ Hmodel₂") as %->.
+          iMod (mpmc_bqueue_model_update (vs ++ [v]) with "Hmodel₁ Hmodel₂") as "(Hmodel₁ & Hmodel₂)".
+          iMod ("HΦ" with "[Hmodel₁]") as "HΦ"; [iSteps.. |].
+          iSplitR "HΦ".
+          { iExists (hist ++ [new_back]), past, front, (nodes ++ [new_back]), back, (vs ++ [v]).
+            iSteps; iPureIntro.
+            - rewrite Hhist -assoc //.
+            - rewrite elem_of_app. naive_solver.
+          }
+          iSteps.
+  Qed.
 
   Lemma mpmc_bqueue_push_spec t ι cap v :
     <<<
@@ -439,7 +860,8 @@ Section mpmc_bqueue_G.
       mpmc_bqueue_push t v @ ↑ι
     <<<
       mpmc_bqueue_model t (if decide (length vs = cap) then vs else vs ++ [v])
-    | RET #(bool_decide (length vs = cap)); True
+    | RET #(bool_decide (length vs = cap));
+      True
     >>>.
   Proof.
   Admitted.
@@ -453,10 +875,73 @@ Section mpmc_bqueue_G.
       mpmc_bqueue_pop t @ ↑ι
     <<<
       mpmc_bqueue_model t (tail vs)
-    | RET head vs; True
+    | RET head vs;
+      True
     >>>.
   Proof.
-  Admitted.
+    iIntros "!> %Φ (%l & %γ & -> & -> & #Hmeta & #Hl_capacity & #Hinv) HΦ".
+
+    iLöb as "HLöb".
+
+    wp_rec.
+    wp_smart_apply (mpmc_bqueue_front_spec with "Hinv") as (old_front i) "(#Hhistory_elem_old & #Hfront_lb_old)".
+    wp_smart_apply (mpmc_bqueue_xchain_next_spec_strong MpmcQueuePop _ inhabitant inhabitant _ [tele_arg] with "[$Hmeta $Hinv $Hhistory_elem_old $Hfront_lb_old $HΦ]") as (res) "[(-> & HΦ) | (%front & -> & #Hhistory_elem & HΦ)]"; [iSteps.. |].
+    wp_pures.
+
+    wp_bind (CAS _ _ _).
+    iInv "Hinv" as "(%hist & %past & %front' & %nodes & %back & %vs & %waiters & >%Hhist & >%Hback & Hl_front & Hl_back & Hhist & Hnodes & Hindexing & >Hhistory_auth & Hfront_auth & Hmodel₂ & Hwaiters_auth & Hwaiters)".
+    iDestruct (mpmc_bqueue_history_agree with "Hhistory_auth Hhistory_elem") as %Hlookup.
+    iDestruct (xchain_model_lookup_acc with "Hhist") as "(Hnode & Hhist)"; first done.
+    wp_cas as _ | [= ->].
+    all: iDestruct ("Hhist" with "Hnode ") as "Hhist".
+
+    - iSplitR "HΦ". { repeat iExists _. iSteps. }
+      iSteps.
+
+    - iDestruct (mpmc_bqueue_history_agree with "Hhistory_auth Hhistory_elem_old") as %Hlookup_old.
+      iAssert ⌜length past = i⌝%I as %Hpast_length.
+      { iDestruct (xchain_model_NoDup with "Hhist") as %Hnodup.
+        iPureIntro. eapply NoDup_lookup; try done.
+        rewrite Hhist list_lookup_middle //.
+      }
+      rewrite Hhist (assoc _ _ [_]) lookup_app_r app_length /= in Hlookup; first lia.
+      rewrite Nat.add_1_r Hpast_length Nat.sub_diag in Hlookup.
+      destruct nodes as [| node nodes]; first done. injection Hlookup as ->.
+      rewrite (assoc _ _ [_]) in Hhist.
+      iDestruct (big_sepL2_cons_inv_l with "Hnodes") as "(%v & %vs' & -> & Hfront_data & Hnodes)".
+      set past' := past ++ [old_front].
+      iMod (mpmc_bqueue_front_update (length past') with "Hfront_auth") as "Hfront_auth".
+      { rewrite app_length. lia. }
+      iDestruct (big_sepM_impl_thread_fupd _ (mpmc_bqueue_waiter γ ι past')%I with "Hwaiters Hmodel₂ [#]") as ">(Hwaiters & Hmodel₂)".
+      { iIntros "!> %waiter %j %Hlookup (%P & #Hwaiter & HP) Hmodel₂".
+        destruct (Nat.lt_trichotomy j (length past)) as [Hj | [-> | Hj]].
+        - rewrite decide_True //.
+          rewrite /mpmc_bqueue_waiter. setoid_rewrite decide_True; last first.
+          { rewrite app_length /=. lia. }
+          iSteps.
+        - rewrite decide_False; first lia.
+          rewrite /mpmc_bqueue_waiter. setoid_rewrite decide_True; last first.
+          { rewrite app_length /=. lia. }
+          iMod "HP" as "(%vs & Hmodel₁ & _ & HP)".
+          iDestruct (mpmc_bqueue_model_agree with "Hmodel₁ Hmodel₂") as %->.
+          iSteps.
+        - rewrite decide_False; first lia.
+          rewrite /mpmc_bqueue_waiter. setoid_rewrite decide_False; last first.
+          { rewrite app_length /=. lia. }
+          iSteps.
+      }
+      iMod "HΦ" as "(%_vs & (%_l & %_γ & %Heq & #_Hmeta & Hmodel₁) & _ & HΦ)". injection Heq as <-.
+      iDestruct (meta_agree with "Hmeta _Hmeta") as %<-. iClear "_Hmeta".
+      iDestruct (mpmc_bqueue_model_agree with "Hmodel₁ Hmodel₂") as %->.
+      iMod (mpmc_bqueue_model_update vs' with "Hmodel₁ Hmodel₂") as "(Hmodel₁ & Hmodel₂)".
+      iMod ("HΦ" with "[Hmodel₁]") as "HΦ"; first iSteps.
+      iSplitR "Hfront_data HΦ".
+      { repeat iExists _. iFrame. iSteps.
+        iApply (big_sepL_impl with "Hindexing").
+        rewrite app_length. iSteps.
+      }
+      iSteps.
+  Qed.
 End mpmc_bqueue_G.
 
 #[global] Opaque mpmc_bqueue_create.
